---
title: "Stat/Math 415 Homework 10"
subtitle: "Due Friday Dec 13; Joseph Sepich (jps6444)"
output:
  pdf_document:
    toc: false
    toc_depth: 2
    number_sections: true
    keep_tex: false
---

# Problem 6.8-1

Problem constraints:

\[Y \sim Poisson(\lambda)\]
\[\theta \sim Gamma(\alpha, \beta)\]

Going off this we have:

\[P(Y=y) = \frac{\lambda^ye^{-\lambda}}{y!}\]
\[f(\theta) = \frac{\theta^{\alpha - 1}e^{-\theta/\beta}}{\Gamma(\alpha)\beta^\alpha}\]

This second pdf would be the prior pdf for our parameter.

## Part a

To get our posterior pdf we must solve for $h(\theta|y)$ where y is our data.

\[h(\theta|y) = \frac{P(y|\theta)f(\theta)}{P(y)} = \frac{P(y|\theta)f(\theta)}{\int P(y|\theta)f(\theta)d\theta}\]
\[\int P(y|\theta)f(\theta)d\theta = \int \frac{n\theta^ye^{-n\theta}}{y!}\frac{\theta^{\alpha - 1}e^{-\theta/\beta}}{\Gamma(\alpha)\beta^\alpha}d\theta\]
\[= \frac{n^y}{y!\Gamma(\alpha)\beta^\alpha} \int \theta^{\alpha + y  - 1}e^{-n\theta-\theta/\beta}d\theta\]
\[= \frac{n^y}{y!\Gamma(\alpha)\beta^\alpha} \int \theta^{\alpha + y  - 1}e^{-\theta(n+1/\beta)}d\theta\]

Now let's multiply by one to make the solution to the integral a trivial one, being a Gamma distribution pdf:

\[= \frac{n^y\Gamma(y + \alpha)(\frac{1}{n + 1/\beta})^{y+\alpha}}{y!\Gamma(\alpha)\beta^\alpha} \int \frac{\theta^{\alpha + y  - 1}e^{-\theta(n+1/\beta)}}{\Gamma(y + \alpha)(\frac{1}{n + 1/\beta})^{y+\alpha}} d\theta\]
\[= \frac{n^y\Gamma(y + \alpha)(\frac{1}{n + 1/\beta})^{y+\alpha}}{y!\Gamma(\alpha)\beta^\alpha}\]
\[= \frac{n^y\Gamma(y + \alpha)}{y!\Gamma(\alpha)\beta^\alpha(n + 1/\beta)^{y + \alpha}} \]
\[= \frac{n^y\Gamma(y + \alpha)\beta^y}{y!\Gamma(\alpha)(n\beta + 1)^{y + \alpha}} \]

Plugging back in to the posterior:

\[h(\theta|y) = \frac{P(y|\theta)f(\theta)}{\int P(y|\theta)f(\theta)d\theta}\]
\[= \frac{\frac{n\theta^ye^{-n\theta}}{y!}\frac{\theta^{\alpha - 1}e^{-\theta/\beta}}{\Gamma(\alpha)\beta^\alpha}}{\frac{n^y\Gamma(y + \alpha)\beta^y}{y!\Gamma(\alpha)(n\beta + 1)^{y + \alpha}}}\]
\[= \frac{\theta^{y + \alpha - 1}e^{-\theta(n + 1/\beta)}}{\Gamma(y + \alpha)(1/(n + 1/\beta))^{y+\alpha}}\]

This means that our posterior distrbution is a Gamma distribution with parameters $\alpha + y$ and $\frac{1}{n + 1/\beta}$.

## Part b

Our loss fuction is $[w(y)-\theta]^2$. We want to find our point estimate w(y), which would be the expected value of our posterior distribution:

\[E[\theta | y] = \alpha + y * \frac{1}{n + 1/\beta} = \frac{y + \alpha}{n + 1/\beta}\]

## Part c

\[w(y) = \frac{y}{n}\frac{n}{(n+1/\beta)} + \frac{\alpha\beta(1/\beta)}{(n + 1/\beta)}\]
\[= \frac{y}{(n+1/\beta)} + \frac{\alpha}{(n + 1/\beta)}\]
\[= \frac{y + \alpha}{n + 1/\beta}\]

This shows that w(y) is the weighted average of the maximum likelihood estimate y/n and the prior mean $\alpha\beta$.

# Problem 6.8-4



# Problem 6.9-1

# Problem Bayesian Decision Exercise

## Part a

## Part b






































